Checkpoint progress removing ephemeral proposal; realized that the
proof still needs an ephemeral proposal, so I'll have to add back in
some version of it. This time, I can do it right and only keep an
ephemeral proposal on the primary and avoid the headache of keeping it
up to date on the backups.

The ephemeral proposal is ghost state to address the following issue:
when the primary gets an "ApplyRo" RPC from the client (e.g. to do a
Get(k) in a KV system), it reads the state from some log `ops1` of
operations which might not yet be durable. These ops might have not
actually been "proposed" in the pb_protocol sense. The pb_protocol
proposal is updated when the ops are made durable.

So, when reading the not-yet-durable list `ops1`, we need the server to
promise that if anything is proposed prior to a crash, the thing that's
proposed is exactly what the ApplyRo thread reads in memory. The
ephemeral proposal tracks the ops that the server has promised it's
going to try really propose in this crash-generation. In terms of this
ephemeral proposal, one can make everything work out (this is how the
heartbeat-based optimization works).

This huge proof complicatoin can be traced to one aspect of the
implementation:
  a server might be the leader in a particular epoch and put some ops in
  its log in memory, crash, restart, get a duplicate RPC telling it to
  become leader in that same epoch, and then put DIFFERENT ops at the
  same place in the in-memory log. This forces the implementation to not
  send RPCs to backups until AFTER the primary makes its state durable.

Maybe it's time to stop doing this, and reduce the normal-case latency
by 1 disk write in exchange for disallowing a server to restart and
continue as primary in the same epoch.

Somehow making this change to the Go code would greatly simplify the
proof and improve performance a bit. I think we know how we might
approach the more complicated proof challenge, having done most of it in
the case of heartbeats using this ephemeral proposal stuff. At this
point, either we should plan to talk about this ephemeral proposal proof
challenge, or tweak the implementation to do away with it and focus on
what we actually care about in the proof.

src/program_proof/simplepb/pb_definitions.v
@@ -32,36 +32,13 @@ Notation has_op_encoding := (Sm.has_op_encoding pb_record).
 Notation has_snap_encoding := (Sm.has_snap_encoding pb_record).
 Notation compute_reply := (Sm.compute_reply pb_record).
 
-Inductive GhostOpType :=
-  | rw_op : OpType → GhostOpType
-  | ro_op : OpType → GhostOpType.
-
 (* opsfull has all the ghost ops (RO and RW) in it as well as the gname for the
    Q for that op. get_rwops returns the RW ops only with the gnames removed.
    Generalizing it to an arbitrary extra type A instead of gname
    specifically, because sometimes we want to use get_rwops on a list that has
    an iProp predicate instead of the gname (see is_inv). *)
-Definition get_rwops {A} (opsfull:list (GhostOpType * A)) : list OpType :=
-  concat (map (λ opfull, match opfull with
-                         | (rw_op op, γ) => [op]
-                         | (ro_op _, _) => []
-                         end) opsfull).
-
-Lemma get_rwops_app {A} (opsfull newops:list (GhostOpType * A)) :
-  get_rwops (opsfull ++ newops) = (get_rwops opsfull) ++ (get_rwops newops).
-Proof.
-  unfold get_rwops.
-  by rewrite map_app concat_app.
-Qed.
-
-Lemma get_rwops_prefix {A} (a b:list (GhostOpType * A)) :
-  prefix a b → prefix (get_rwops a) (get_rwops b).
-Proof.
-  intros Hprefix.
-  destruct Hprefix as [c ->].
-  rewrite get_rwops_app.
-  by apply prefix_app_r.
-Qed.
+Definition get_rwops {A} (opsfull:list (OpType * A)) : list OpType :=
+  fst <$> opsfull.
 
 Definition client_logR := mono_listR (leibnizO OpType).
 
@@ -69,7 +46,7 @@ Class pbG Σ := {
     (*
     pb_ghostG :> pb_ghostG (EntryType:=(OpType * (list OpType → iProp Σ))%type) Σ ;
      *)
-    pb_ghostG :> pb_ghostG (EntryType:=(GhostOpType * gname)) Σ ;
+    pb_ghostG :> pb_ghostG (EntryType:=(OpType * gname)) Σ ;
     pb_savedG :> savedPredG Σ (list OpType);
     pb_urpcG :> urpcregG Σ ;
     pb_wgG :> waitgroupG Σ ; (* for apply proof *)
@@ -78,7 +55,7 @@ Class pbG Σ := {
 }.
 
 Definition pbΣ :=
-  #[pb_ghostΣ (EntryType:=(GhostOpType * gname)); savedPredΣ (list OpType) ; urpcregΣ ; waitgroupΣ ;
+  #[pb_ghostΣ (EntryType:=(OpType * gname)); savedPredΣ (list OpType) ; urpcregΣ ; waitgroupΣ ;
     GFunctor (client_logR) ; ghost_varΣ unit].
 Global Instance subG_pbΣ {Σ} : subG (pbΣ) Σ → (pbG Σ).
 Proof. solve_inG. Qed.
@@ -93,7 +70,7 @@ Definition own_log γ σ := own γ (●ML{#1/2} (σ : list (leibnizO OpType))).
 Definition ApplyAsBackup_core_spec γ γsrv args opsfull op Q (Φ : u64 -> iProp Σ) : iProp Σ :=
   ("%Hσ_index" ∷ ⌜length (get_rwops opsfull) = (int.nat args.(ApplyAsBackupArgs.index) + 1)%nat⌝ ∗
    "%Hhas_encoding" ∷ ⌜has_op_encoding args.(ApplyAsBackupArgs.op) op⌝ ∗
-   "%Hghost_op_σ" ∷ ⌜last opsfull = Some (rw_op op, Q)⌝ ∗
+   "%Hghost_op_σ" ∷ ⌜last opsfull = Some (op, Q)⌝ ∗
    "%Hno_overflow" ∷ ⌜int.nat args.(ApplyAsBackupArgs.index) < int.nat (word.add args.(ApplyAsBackupArgs.index) 1)⌝ ∗
    "#Hepoch_lb" ∷ is_epoch_lb γsrv args.(ApplyAsBackupArgs.epoch) ∗
    "#Hprop_lb" ∷ is_proposal_lb γ args.(ApplyAsBackupArgs.epoch) opsfull ∗
@@ -200,8 +177,8 @@ Defined.
 Definition appN := pbN .@ "app".
 Definition escrowN := pbN .@ "escrow".
 
-Definition own_ghost' γsys (opsfullQ : list (GhostOpType * (list OpType → iProp Σ))) : iProp Σ :=
-  ∃ ops_gnames: list (GhostOpType * gname),
+Definition own_ghost' γsys (opsfullQ : list (OpType * (list OpType → iProp Σ))) : iProp Σ :=
+  ∃ ops_gnames: list (OpType * gname),
     own_ghost γsys ops_gnames ∗
     ⌜opsfullQ.*1 = ops_gnames.*1 ⌝ ∗
     [∗ list] k↦Φ;γ ∈ snd <$> opsfullQ; snd <$> ops_gnames, saved_pred_own γ DfracDiscarded Φ.
@@ -240,28 +217,6 @@ Next Obligation.
   solve_proper.
 Defined.
 
-Definition RoApplyAsBackup_core_spec γ γsrv args opsfull (Φ : u64 -> iProp Σ) : iProp Σ :=
-  ("%Hσ_index" ∷ ⌜length (get_rwops opsfull) = (int.nat args.(RoApplyAsBackupArgs.nextIndex))%nat⌝ ∗
-   "#Hepoch_lb" ∷ is_epoch_lb γsrv args.(RoApplyAsBackupArgs.epoch) ∗
-   "#Hprop_lb" ∷ is_proposal_lb γ args.(RoApplyAsBackupArgs.epoch) opsfull ∗
-   "#Hprop_facts" ∷ is_proposal_facts γ args.(RoApplyAsBackupArgs.epoch) opsfull ∗
-   "HΨ" ∷ ((is_accepted_lb γsrv args.(RoApplyAsBackupArgs.epoch) opsfull -∗ Φ (U64 0)) ∧
-           (∀ (err:u64), ⌜err ≠ 0⌝ -∗ Φ err))
-    )%I
-.
-
-Program Definition RoApplyAsBackup_spec γ γsrv :=
-  λ (encoded_args:list u8), λne (Φ : list u8 -d> iPropO Σ) ,
-  (∃ args opsfull,
-    ⌜RoApplyAsBackupArgs.has_encoding encoded_args args⌝ ∗
-    RoApplyAsBackup_core_spec γ γsrv args opsfull (λ err, ∀ reply, ⌜reply = u64_le err⌝ -∗ Φ reply)
-    )%I
-.
-Next Obligation.
-  unfold RoApplyAsBackup_core_spec.
-  solve_proper.
-Defined.
-
 Definition ApplyRo_core_spec γ γlog op enc_op :=
   λ (Φ : ApplyReply.C -> iPropO Σ) ,
   (
@@ -286,7 +241,6 @@ Next Obligation.
 Defined.
 
 
-
 Definition is_pb_host_pre ρ : (u64 -d> pb_system_names -d> pb_server_names -d> iPropO Σ) :=
   (λ host γ γsrv,
   ∃ γrpc,
@@ -295,9 +249,8 @@ Definition is_pb_host_pre ρ : (u64 -d> pb_system_names -d> pb_server_names -d> 
   handler_spec γrpc host (U64 2) (GetState_spec γ γsrv) ∗
   handler_spec γrpc host (U64 3) (BecomePrimary_spec_pre γ γsrv ρ) ∗
   handler_spec γrpc host (U64 4) (Apply_spec γ) ∗
-  handler_spec γrpc host (U64 5) (RoApplyAsBackup_spec γ γsrv) ∗
   handler_spec γrpc host (U64 6) (ApplyRo_spec γ) ∗
-  handlers_dom γrpc {[ (U64 0) ; (U64 1) ; (U64 2) ; (U64 3) ; (U64 4) ; (U64 5) ; (U64 6) ]})%I
+  handlers_dom γrpc {[ (U64 0) ; (U64 1) ; (U64 2) ; (U64 3) ; (U64 4) ; (U64 6) ]})%I
 .
 
 Instance is_pb_host_pre_contr : Contractive is_pb_host_pre.
@@ -332,39 +285,15 @@ Qed.
 
 (* End RPC specs *)
 
-Definition own_ephemeral_proposal γeph (epoch:u64) (opsfull:list (GhostOpType * gname)) : iProp Σ :=
-  epoch ⤳l[γeph] opsfull.
-
-Definition is_ephemeral_proposal_lb γeph (epoch:u64) (opsfull:list (GhostOpType * gname)) : iProp Σ :=
-  epoch ⤳l[γeph]⪰ opsfull.
-
-Definition is_ephemeral_proposal_sealed γeph (epoch:u64) (opsfull:list (GhostOpType * gname)) : iProp Σ :=
-  epoch ⤳l[γeph]□ opsfull.
-
-Definition own_unused_ephemeral_proposals γeph (epoch:u64) : iProp Σ :=
-  [∗ set] epoch' ∈ (fin_to_set u64), ⌜int.nat epoch' <= int.nat epoch⌝ ∨ own_ephemeral_proposal γeph epoch' []
-.
-
 (* Encapsulates the protocol-level ghost resources of a replica server; this is
    suitable for exposing as part of interfaces for users of the library. For
    now, it's only part of the crash obligation. *)
 (* should not be unfolded in proof *)
-Definition own_Server_ghost_f γ γsrv γeph epoch ops sealed : iProp Σ :=
+Definition own_Server_ghost_f γ γsrv epoch ops sealed : iProp Σ :=
   ∃ opsfull,
   "%Hre" ∷ ⌜ops = get_rwops opsfull⌝ ∗
-  "#Heph_lb" ∷ is_ephemeral_proposal_lb γeph epoch opsfull ∗
-  (* XXX: this ephemeral_proposal is really only used on the primary. The
-     invariant could maintain this only in the case that the server is primary,
-     but then we would need to prove that a server is definitely not primary
-     when it gets an ApplyAsBackup RPC. To avoid that annoyance, the proof keeps
-     this everywhere *)
   "Hghost" ∷ (own_replica_ghost γ γsrv epoch opsfull sealed) ∗
-  "Hprim" ∷ (own_primary_ghost γ γsrv epoch opsfull) ∗
-  "#Heph_sealed" ∷ □(if sealed then (∃ opsfull_ephemeral, is_ephemeral_proposal_sealed γeph epoch opsfull_ephemeral) else True)
-  (* XXX: keeping sealed ephemeral proposal so that:
-     when the primary is NOT sealed, it will have own_proposal, which tells it
-     that the server cannot be sealed.
-   *)
+  "Hprim" ∷ (own_primary_ghost γ γsrv epoch opsfull)
 .
 
 End pb_global_definitions.
@@ -374,19 +303,15 @@ Record t {pb_record:Sm.t} :=
   mkC {
     epoch : u64 ;
     sealed : bool ;
-    ops_full_eph: list (GhostOpType (pb_record:=pb_record) * gname) ;
+    ops_full_eph: list (pb_record.(Sm.OpType) * gname) ;
     isPrimary : bool ;
-    durableNextIndex : u64 ;
 
     (* read-only optimization-related *)
     committedNextIndex : u64 ;
-    nextRoIndex : u64 ;
-    committedNextRoIndex : u64 ;
   }.
 
 Global Instance etaServer {pb_record:Sm.t} : Settable _ :=
-  settable! (mkC pb_record) <epoch; sealed; ops_full_eph; isPrimary; durableNextIndex;
-committedNextIndex; nextRoIndex; committedNextRoIndex>.
+  settable! (mkC pb_record) <epoch; sealed; ops_full_eph; isPrimary; committedNextIndex>.
 End server.
 
 Section pb_local_definitions.
@@ -524,10 +449,10 @@ Qed.
 
 Definition numClerks : nat := 32.
 
-Notation GhostOpType := (GhostOpType (pb_record:=pb_record)).
 Notation get_rwops := (get_rwops (pb_record:=pb_record)).
 
-Definition is_full_ro_suffix {A:Type} r (l:list (GhostOpType * A)) :=
+(*
+Definition is_full_ro_suffix {A:Type} r (l:list (OpType * A)) :=
   ∀ r',
   get_rwops r' = [] →
   suffix r' l →
@@ -542,7 +467,7 @@ Admitted.
 
 (* FIXME: move these lemmas *)
 Lemma is_full_ro_suffix_nil {A} l op a:
-      is_full_ro_suffix (A:=A) [] (l ++ [(rw_op op, a)]).
+      is_full_ro_suffix (A:=A) [] (l ++ [(op, a)]).
 Proof.
   intros r Hros Hsuffix.
   destruct (decide (length r = 0)).
@@ -593,7 +518,7 @@ Qed.
    leph ends with 5 RO ops.
    Want to derive contradiction.
  *)
-Lemma roapply_helper {A} r l r' (l':list (GhostOpType * A)) :
+Lemma roapply_helper {A} r l r' (l':list (OpType * A)) :
   is_full_ro_suffix r l →
   is_full_ro_suffix r' l' →
   prefix l' l →
@@ -604,7 +529,7 @@ Lemma roapply_helper {A} r l r' (l':list (GhostOpType * A)) :
 .
 Proof.
   intros Hcontains Hcontains' Hprefix' Hrws Hsuffix' Hros.
-Admitted.
+Admitted. *)
 
 (* this is meant to be unfolded in the code proof *)
 Definition is_Primary γ γsrv (s:server.t) clerks_sl : iProp Σ:=
@@ -622,34 +547,21 @@ Definition is_Primary γ γsrv (s:server.t) clerks_sl : iProp Σ:=
 .
 
 (* this should never be unfolded in the proof of code *)
-Definition is_Primary_ghost_f γ γeph γsrv (st:server.t): iProp Σ:=
+Definition is_Primary_ghost_f γ γsrv epoch (committedNextIndex nextIndex:u64) : iProp Σ:=
   tc_opaque (
-            ∃ (ops_commit_full:list (GhostOpType * gname)),
-            "#Htok_used_witness" ∷ is_tok γsrv st.(server.epoch) ∗
+            ∃ (ops_commit_full:list (OpType * gname)),
+            "#Htok_used_witness" ∷ is_tok γsrv epoch ∗
 
             (* committed witness for committed state *)
             "#Hcommit_lb" ∷ is_ghost_lb γ ops_commit_full ∗
-            "#Heph_commit_lb" ∷ is_ephemeral_proposal_lb γeph st.(server.epoch) ops_commit_full ∗
-            "%HcommitLen" ∷ ⌜int.nat st.(server.committedNextIndex) ≤ int.nat (length (get_rwops st.(server.ops_full_eph)))⌝ ∗
-            "%HcommitRoNz" ∷ ⌜int.nat st.(server.committedNextIndex) < int.nat (length (get_rwops st.(server.ops_full_eph))) → int.nat st.(server.committedNextRoIndex) = 0⌝ ∗
+            "%HcommitLen" ∷ ⌜int.nat committedNextIndex ≤ int.nat nextIndex⌝ ∗
 
-            (* opsfull_eph has `nextRoIndex` RO ops as its tail. *)
-            "%HcommitLen" ∷ ⌜length (get_rwops ops_commit_full) = int.nat st.(server.committedNextIndex)⌝ ∗
-            "%Heph_proposal" ∷ ⌜∃ opsfull_eph_ro,
-                                suffix opsfull_eph_ro st.(server.ops_full_eph) ∧
-                                length opsfull_eph_ro = int.nat st.(server.nextRoIndex) ∧
-                                get_rwops opsfull_eph_ro = [] ∧
-                                is_full_ro_suffix opsfull_eph_ro st.(server.ops_full_eph)⌝ ∗
-            "%HcommitRoLen" ∷ ⌜ ∃ ops_commit_ro,
-                                suffix ops_commit_ro ops_commit_full ∧
-                                length ops_commit_ro >= int.nat st.(server.committedNextRoIndex) ∧
-                                get_rwops ops_commit_ro = [] ∧
-                                is_full_ro_suffix ops_commit_ro ops_commit_full⌝
+            "%HcommitLen" ∷ ⌜length (get_rwops ops_commit_full) = int.nat committedNextIndex⌝
       )%I
 .
 
-Global Instance is_Primary_ghost_pers γ γeph γsrv st:
-  Persistent (is_Primary_ghost_f γ γeph γsrv st).
+Global Instance is_Primary_ghost_pers γ γsrv epoch committedNextIndex nextIndex:
+  Persistent (is_Primary_ghost_f γ γsrv epoch committedNextIndex nextIndex).
 Proof.
 unfold is_Primary_ghost_f. unfold tc_opaque. apply _.
 Qed.
@@ -658,10 +570,9 @@ Definition no_overflow (x:nat) : Prop := int.nat (U64 x) = x.
 Hint Unfold no_overflow : arith.
 
 (* physical (volatile) state; meant to be unfolded in code proof *)
-Definition own_Server (s:loc) (st:server.t) γ γsrv mu γeph: iProp Σ :=
+Definition own_Server (s:loc) (st:server.t) γ γsrv mu : iProp Σ :=
   ∃ own_StateMachine (sm:loc) clerks_sl
-    (roOpsToPropose_cond committedNextRoIndex_cond durableNextIndex_cond:loc)
-    (opAppliedConds_loc:loc) (opAppliedConds:gmap u64 loc),
+    (committedNextIndex_cond:loc) (opAppliedConds_loc:loc) (opAppliedConds:gmap u64 loc),
   (* non-persistent physical *)
   "Hepoch" ∷ s ↦[pb.Server :: "epoch"] #st.(server.epoch) ∗
   "HnextIndex" ∷ s ↦[pb.Server :: "nextIndex"] #(U64 (length (get_rwops st.(server.ops_full_eph)))) ∗
@@ -669,91 +580,51 @@ Definition own_Server (s:loc) (st:server.t) γ γsrv mu γeph: iProp Σ :=
   "Hsealed" ∷ s ↦[pb.Server :: "sealed"] #st.(server.sealed) ∗
   "Hsm" ∷ s ↦[pb.Server :: "sm"] #sm ∗
   "Hclerks" ∷ s ↦[pb.Server :: "clerks"] (slice_val clerks_sl) ∗
-  "HdurableNextIndex" ∷ s ↦[pb.Server :: "durableNextIndex"] #st.(server.durableNextIndex) ∗
-  "HdurableNextIndex_cond" ∷ s ↦[pb.Server :: "durableNextIndex_cond"] #durableNextIndex_cond ∗
   "HcommittedNextIndex" ∷ s ↦[pb.Server :: "committedNextIndex"] #st.(server.committedNextIndex) ∗
-  "HnextRoIndex" ∷ s ↦[pb.Server :: "nextRoIndex"] #st.(server.nextRoIndex) ∗
-  "HcommittedNextRoIndex" ∷ s ↦[pb.Server :: "committedNextRoIndex"] #st.(server.committedNextRoIndex) ∗
-  "HroOpsToPropose_cond" ∷ s ↦[pb.Server :: "roOpsToPropose_cond"] #roOpsToPropose_cond ∗
-  "HcommittedNextRoIndex_cond" ∷ s ↦[pb.Server :: "committedNextRoIndex_cond"] #committedNextRoIndex_cond ∗
+  "HcommittedNextIndex_cond" ∷ s ↦[pb.Server :: "committedNextIndex_cond"] #committedNextIndex_cond ∗
   (* backup sequencer *)
   "HopAppliedConds" ∷ s ↦[pb.Server :: "opAppliedConds"] #opAppliedConds_loc ∗
   "HopAppliedConds_map" ∷ is_map opAppliedConds_loc 1 opAppliedConds ∗
 
   (* ownership of the statemachine *)
-  "Hstate" ∷ own_StateMachine st.(server.epoch) (get_rwops st.(server.ops_full_eph)) st.(server.sealed) (own_Server_ghost_f γ γsrv γeph) ∗
+  "Hstate" ∷ own_StateMachine st.(server.epoch) (get_rwops st.(server.ops_full_eph)) st.(server.sealed) (own_Server_ghost_f γ γsrv) ∗
 
   (* persistent physical state *)
   "#HopAppliedConds_conds" ∷ ([∗ map] i ↦ cond ∈ opAppliedConds, is_cond cond mu) ∗
-  "#HdurableNextIndex_is_cond" ∷ is_cond durableNextIndex_cond mu ∗
-  "#HroOpsToPropose_is_cond" ∷ is_cond roOpsToPropose_cond mu ∗
-  "#HcommittedNextRoIndex_is_cond" ∷ is_cond committedNextRoIndex_cond mu ∗
+  "#HcommittedNextRoIndex_is_cond" ∷ is_cond committedNextIndex_cond mu ∗
 
   (* witnesses for primary; the exclusive state is in own_Server_ghost *)
   "#Hprimary" ∷ (⌜st.(server.isPrimary) = false⌝ ∨ is_Primary γ γsrv st clerks_sl) ∗
 
   (* state-machine callback specs *)
-  "#HisSm" ∷ is_StateMachine sm own_StateMachine (own_Server_ghost_f γ γsrv γeph) ∗
+  "#HisSm" ∷ is_StateMachine sm own_StateMachine (own_Server_ghost_f γ γsrv) ∗
 
   (* overflow *)
   "%HnextIndexNoOverflow" ∷ ⌜no_overflow (length (get_rwops (st.(server.ops_full_eph))))⌝
 .
 
 (* should not be unfolded in proof *)
-Definition own_Server_ghost_eph_f (st:server.t) γ γsrv γeph : iProp Σ :=
+Definition own_Server_ghost_eph_f (st:server.t) γ γsrv: iProp Σ :=
   tc_opaque (
   let ops:=(get_rwops st.(server.ops_full_eph)) in
-  ∃ ops_durable_full,
-  (* non-persistent ghost state *)
-  "Heph" ∷ (if st.(server.sealed) then
-              is_ephemeral_proposal_sealed γeph st.(server.epoch) st.(server.ops_full_eph)
-            else
-              own_ephemeral_proposal γeph st.(server.epoch) st.(server.ops_full_eph)) ∗
-  "Heph_unused" ∷ own_unused_ephemeral_proposals γeph st.(server.epoch) ∗
-
   (* epoch lower bound *)
   "#Hs_epoch_lb" ∷ is_epoch_lb γsrv st.(server.epoch) ∗
 
-  (* persistent ghost-state *)
-  "#Heph_prop_lb" ∷ □(if st.(server.isPrimary) then True else is_proposal_lb γ st.(server.epoch) st.(server.ops_full_eph)) ∗
-  (* accepted witness for durable state *)
-  "#Hdurable_lb" ∷ is_accepted_lb γsrv st.(server.epoch) ops_durable_full ∗
-  "#Hdurable_eph_lb" ∷ is_ephemeral_proposal_lb γeph st.(server.epoch) ops_durable_full ∗
-  "#Heph_valid" ∷ is_proposal_valid γ st.(server.ops_full_eph) ∗
-
-  "%HdurableLen" ∷ ⌜length (get_rwops ops_durable_full) = int.nat st.(server.durableNextIndex)⌝ ∗
-
-  (* `committedRoNextIndex` read-only ops have been committed *)
-
-  (* Want to add pure invariant: nextIndex ≠ committedNextIndex → committedNextRoIndex = 0.
-     Q: Is this invariant true?
-     A: No. ApplyRoThread increases committedNextRoIndex without increasing
-     committedNextIndex (even though it provably could also increase that).
-     Let's suppose we don't change the impl to make this part of the proof
-     easier.
-
-     Here's what *is* true. The first (committedNextRoIndex) ops of the
-     (nextRoIndex) ro ops are committed. To maintain that, need another
-     committed list. This list has an ephemeral_lb (so it agres with
-     opsfull_eph), has all the same RW ops as opsfull_eph, and has
-     committedNextRoIndex RO ops as suffix.
-   *)
-
   (* primary-only *)
-  "#HprimaryOnly" ∷ (⌜st.(server.isPrimary) = false⌝ ∨ is_Primary_ghost_f γ γeph γsrv st)
+  "#HprimaryOnly" ∷ (⌜st.(server.isPrimary) = false⌝ ∨ is_Primary_ghost_f γ γsrv st.(server.epoch) st.(server.committedNextIndex) (U64 (length $ get_rwops st.(server.ops_full_eph))))
   )%I
 .
 
-Definition mu_inv (s:loc) γ γsrv γeph mu: iProp Σ :=
+Definition mu_inv (s:loc) γ γsrv mu: iProp Σ :=
   ∃ st,
-  "Hvol" ∷ own_Server s st γ γsrv mu γeph ∗
-  "HghostEph" ∷ own_Server_ghost_eph_f st γ γsrv γeph
+  "Hvol" ∷ own_Server s st γ γsrv mu ∗
+  "HghostEph" ∷ own_Server_ghost_eph_f st γ γsrv
 .
 
 Definition is_Server (s:loc) γ γsrv : iProp Σ :=
-  ∃ (mu:val) γeph,
+  ∃ (mu:val),
   "#Hmu" ∷ readonly (s ↦[pb.Server :: "mu"] mu) ∗
-  "#HmuInv" ∷ is_lock pbN mu (mu_inv s γ γsrv γeph mu) ∗
+  "#HmuInv" ∷ is_lock pbN mu (mu_inv s γ γsrv mu) ∗
   "#Hsys_inv" ∷ sys_inv γ.
 
 Lemma wp_Server__isEpochStale {stk} (s:loc) (currEpoch epoch:u64) :
